Clean up the termination condition for LoopIncI32
By changing it to more closely match LoopBase, this change makes it
easier to apply theorems on the base class to an instance of LoopIncI32.

Also, I removed a big block of commented-out code from Loops.lean
that I had somehow previously missed. Oops!

FormalVerifyMisc/Loops.lean
@@ -22,17 +22,18 @@ alias LoopReverse := LoopBase
 
 -- Loop which continues until some parameter (of type 'β') exceeds some upper bound
 -- 'β' is typically of type Int32, Int64, UInt32, or UInt64
-class LoopForward (α : Type) (β : outParam Type) [LE β] where
+class LoopForward (α : Type) (β : outParam Type)
+  [LE β] [DecidableRel (· ≤ · : β → β → Prop)] where
   -- Upper bound for loop execution
   bound : α → β
   -- A map from the current loop state to β - used to check for termination
   finc : α → β
   -- Function for advancing the loop state
-  fadv : (s : α) → ¬bound s ≤ finc s → α
+  fadv : (s : α) → ¬decide (bound s ≤ finc s) = true → α
   -- Proof that 'finc' increases as 'fadv' is called repeatedly
-  hinc : ∀ s, (h : ¬bound s ≤ finc s) → ¬finc (fadv s h) ≤ finc s
+  hinc : ∀ s h, ¬finc (fadv s h) ≤ finc s
   -- Proof that the bound doesn't change as 'fadv' is called
-  hbound : ∀ s, (h : ¬bound s ≤ finc s) → bound (fadv s h) = bound s
+  hbound : ∀ s h, bound (fadv s h) = bound s
 
 -- A mapping from a type 'β' to the natural numbers
 -- Used in proving loop termination
@@ -71,13 +72,12 @@ instance (α β : Type)
   [LE β] [DecidableRel (· ≤ · : β → β → Prop)]
   [TerminationParam β] [LoopForward α β] : LoopBase α where
   term := fun s ↦ decide (LoopForward.bound s ≤ LoopForward.finc s)
-  adv := fun s h ↦ LoopForward.fadv s (by simp at h; assumption)
+  adv := LoopForward.fadv
   fdec := fun s ↦
     TerminationParam.embed (LoopForward.bound s) -
     TerminationParam.embed (LoopForward.finc s)
   hdec := by
     intro s h
-    simp only [decide_eq_true_eq] at h
     rw [LoopForward.hbound]
     by_contra! h'
     let embed : β ↪o ℕ := TerminationParam.embed
@@ -87,8 +87,9 @@ instance (α β : Type)
       exact embed.map_rel_iff'.mp (Nat.le_of_sub_le_sub_left hle h')
     rename' hle => hlt; push_neg at hlt
     rw [Nat.sub_eq_zero_of_le (le_of_lt hlt)] at h'
-    have hsubzero := Nat.le_of_sub_eq_zero (Nat.eq_zero_of_le_zero h')
-    exact h (embed.map_rel_iff'.mp hsubzero)
+    simp only [decide_eq_true_eq] at h
+    apply h (embed.map_rel_iff'.mp _)
+    exact Nat.le_of_sub_eq_zero (Nat.eq_zero_of_le_zero h')
 
 -- A loop that advances by incrementing a 32-bit integer
 class LoopIncI32 (α : Type) where
@@ -100,7 +101,7 @@ class LoopIncI32 (α : Type) where
   -- The loop will exit if 'cur' ever meets or exceeds 'finish'
   finish : α → Int32
   -- Function for advancing the state
-  adv : (s : α) → cur s < finish s → α
+  adv : (s : α) → ¬decide (finish s ≤ cur s) = true → α
   -- 'inc' must be positive
   hpos : ∀ (s : α), 0 < (inc s)
   -- A proof that the loop execution will not exceed the 32-bit limit
@@ -128,11 +129,11 @@ lemma loop_incI32_toInt_val_add_inc {α : Type} [LoopIncI32 α] (s : α)
 
 -- In particular, 'cur + inc' can be moved across the 'toInt' conversion
 lemma loop_incI32_toInt_cur_add_inc {α : Type} [LoopIncI32 α] (s : α)
-  (h : ¬LoopIncI32.finish s ≤ LoopIncI32.cur s) :
+  (h : LoopIncI32.cur s < LoopIncI32.finish s) :
   (LoopIncI32.cur s + LoopIncI32.inc s).toInt =
   (LoopIncI32.cur s).toInt + (LoopIncI32.inc s).toInt := by
   apply loop_incI32_toInt_val_add_inc
-  exact Int32.le_of_lt (Int32.not_le.mp h)
+  exact Int32.le_of_lt h
 
 -- In particular, 'finish + inc' can be moved across the 'toInt' conversion
 lemma loop_incI32_toInt_finish_add_inc {α : Type} [LoopIncI32 α] (s : α) :
@@ -145,16 +146,17 @@ lemma loop_incI32_toInt_finish_add_inc {α : Type} [LoopIncI32 α] (s : α) :
 instance (α : Type) [LoopIncI32 α] : LoopForward α Int32 where
   bound := LoopIncI32.finish
   finc := LoopIncI32.cur
-  fadv := fun s h ↦ LoopIncI32.adv s (Int32.not_le.mp h)
+  fadv := fun s h ↦ LoopIncI32.adv s h
   hinc := by
     intro s h
+    simp only [decide_eq_true_eq, Int32.not_le] at h
     rw [LoopIncI32.hadv, Int32.not_le]
     have incpos := Int32.lt_iff_toInt_lt.mp (LoopIncI32.hpos s)
     have := Int.add_lt_add_left incpos (LoopIncI32.cur s).toInt
     rw [Int32.toInt_zero, add_zero] at this
     apply Int32.lt_iff_toInt_lt.mpr
     rwa [loop_incI32_toInt_cur_add_inc s h]
-  hbound := fun s h ↦ LoopIncI32.hfinish s (Int32.not_le.mp h)
+  hbound := fun s h ↦ LoopIncI32.hfinish s h
 
 -- If a property of the loop state is constant across calls to 'adv'
 -- it will be constant over the full execution of the loop
@@ -204,9 +206,7 @@ decreasing_by
   [TerminationParam β] [LoopForward α β] (s : α) :
   LoopForward.bound (do_loop s) = LoopForward.bound s := by
   apply loop_val_const
-  intro t h
-  simp only [LoopBase.term, decide_eq_true_eq] at h
-  exact LoopForward.hbound t h
+  exact LoopForward.hbound
 
 -- After the execution of a forward loop,
 -- the termination parameter will have exceeded the bound
@@ -247,198 +247,12 @@ theorem loop_incI32_term_param_lt_of_lt {α : Type} [LoopIncI32 α] (s : α)
   have step : ∀ t h, prop t → prop (LoopIncI32.adv t h) := by
     unfold prop
     intro t hterm curlt'
+    simp only [decide_eq_true_eq, Int32.not_le] at hterm
     rw [LoopIncI32.hadv]
     apply Int32.lt_iff_toInt_lt.mpr
     rw [loop_incI32_toInt_finish_add_inc]
-    rw [loop_incI32_toInt_cur_add_inc _ (Int32.not_le.mpr hterm)]
+    rw [loop_incI32_toInt_cur_add_inc _ hterm]
     rw [LoopIncI32.hfinish, LoopIncI32.hinc]
     exact Int.add_lt_add_right (Int32.lt_iff_toInt_lt.mp hterm) _
   rw [← loop_incI32_finish_const, ← loop_incI32_inc_const]
-  apply loop_prop_const _ prop base _
-  intro t hterm hpt
-  simp only [LoopBase.term, decide_eq_true_eq] at hterm
-  exact step t (Int32.not_le.mp hterm) hpt
-
-/-class SimpleLoopState (α : Type) where
-  -- Variable to track our progress through the loop
-  cur : α → Int32
-  -- Amount by which to increment 'cur' on each iteration
-  inc : α → Int32
-  -- Upper bound for the loop
-  -- The loop will exit if 'cur' ever meets or exceeds 'finish'
-  finish : α → Int32
-  -- Function for advancing the state
-  adv : (s : α) → (cur s < finish s) → α
-  -- 'inc' must be positive
-  hpos : ∀ (s : α), 0 < (inc s)
-  -- A proof that the loop execution will not exceed the 32-bit limit
-  hsafe : ∀ (s : α), (finish s).toInt + (inc s).toInt ≤ Int32.maxValue.toInt
-  -- Proof that 'adv' increments 'cur' as long as 'cur' < 'finish'
-  hadv : ∀ s hlt, cur (adv s hlt) = cur s + inc s
-  -- Proof that advancing the state doesn't change 'inc'
-  hinc : ∀ s hlt, inc (adv s hlt) = inc s
-  -- Proof that advancing the state doesn't change 'finish'
-  hfinish : ∀ s hlt, finish (adv s hlt) = finish s
-
--- Map the 32-bit integers to the natural numbers
--- for the purpose of proving termination
-def int32_toNat_for_term (i : Int32) : ℕ := (i.toInt + 2 ^ 31).natAbs
-
--- Converting a 32-bit integer to ℤ and adding 2^31 results in a non-negative value
-lemma int32_toInt_add_maxValue_nonneg (i : Int32) :
-  0 ≤ i.toInt + 2 ^ 31 := by
-  apply Int.le_add_of_sub_right_le
-  exact int32_minval_le_toInt i
-
--- Prove that the mapping from Int32 to ℕ preserves order
-lemma int32_toNat_for_term_lt_iff (i j : Int32) :
-  i < j ↔ int32_toNat_for_term i < int32_toNat_for_term j := by
-  unfold int32_toNat_for_term
-  have hrwi := Int.ofNat_natAbs_of_nonneg (int32_toInt_add_maxValue_nonneg i)
-  have hrwj := Int.ofNat_natAbs_of_nonneg (int32_toInt_add_maxValue_nonneg j)
-  constructor
-  · intro hlt
-    apply Int.lt_of_ofNat_lt_ofNat
-    rw [hrwi, hrwj]
-    exact Int.add_lt_add_right (Int32.lt_iff_toInt_lt.mp hlt) (2 ^ 31)
-  · intro hlt
-    apply Int32.lt_iff_toInt_lt.mpr
-    apply Int.ofNat_lt_ofNat_of_lt at hlt
-    rw [hrwi, hrwj] at hlt
-    exact Int.lt_of_add_lt_add_right hlt
-
--- This result will be useful for proving that the loop terminates,
--- but will also be useful for clients of this code in proving that
--- loop state constraints are maintained.
-theorem simple_loop_state_toInt_cur_add_inc {α : Type} [SimpleLoopState α] (s : α)
-  (hlt : SimpleLoopState.cur s < SimpleLoopState.finish s) :
-  (SimpleLoopState.cur s + SimpleLoopState.inc s).toInt =
-  (SimpleLoopState.cur s).toInt + (SimpleLoopState.inc s).toInt := by
-  have hpos : (0 : ℤ) < _ := Int32.lt_iff_toInt_lt.mp (SimpleLoopState.hpos s)
-  rw [int32_toInt_add_of_bounds]
-  constructor
-  · exact Int.add_le_add (int32_minval_le_toInt _) (le_of_lt hpos)
-  · have hlt' := Int32.lt_iff_toInt_lt.mp hlt
-    let inc := SimpleLoopState.inc s
-    apply lt_of_lt_of_le (Int.add_lt_add_right hlt' inc.toInt)
-    apply le_trans (SimpleLoopState.hsafe s)
-    rw [Int32.maxValue]; simp
-
--- The addition of 'finish' and 'inc' can be carried across the 'toInt' conversion
-theorem simple_loop_state_toInt_finish_add_inc {α : Type} [SimpleLoopState α] (s : α) :
-  (SimpleLoopState.finish s + SimpleLoopState.inc s).toInt =
-  (SimpleLoopState.finish s).toInt + (SimpleLoopState.inc s).toInt := by
-  have hpos : (0 : ℤ) < _ := Int32.lt_iff_toInt_lt.mp (SimpleLoopState.hpos s)
-  convert int32_toInt_add_of_bounds _ _ _
-  constructor
-  · have ltfin := int32_minval_le_toInt (SimpleLoopState.finish s)
-    linarith [ltfin, hpos]
-  · apply lt_of_le_of_lt (SimpleLoopState.hsafe s)
-    unfold Int32.maxValue; simp
-
--- Prove termination for 'do_simple_loop'
-lemma simple_loop_term {α : Type} [SimpleLoopState α] (s : α)
-  (hlt : SimpleLoopState.cur s < SimpleLoopState.finish s) :
-  int32_toNat_for_term (SimpleLoopState.finish (SimpleLoopState.adv s hlt)) -
-  int32_toNat_for_term (SimpleLoopState.cur (SimpleLoopState.adv s hlt)) <
-  int32_toNat_for_term (SimpleLoopState.finish s) -
-  int32_toNat_for_term (SimpleLoopState.cur s) := by
-  have hpos : (0 : ℤ) < _ := Int32.lt_iff_toInt_lt.mp (SimpleLoopState.hpos s)
-  rw [SimpleLoopState.hfinish s]
-  apply Nat.sub_lt_sub_left ((int32_toNat_for_term_lt_iff _ _).mp hlt)
-  rw [SimpleLoopState.hadv s]
-  apply Int.lt_of_ofNat_lt_ofNat
-  unfold int32_toNat_for_term
-  repeat rw [Int.ofNat_natAbs_of_nonneg (int32_toInt_add_maxValue_nonneg _)]
-  apply Int.add_lt_add_right
-  rw [simple_loop_state_toInt_cur_add_inc _ hlt]
-  apply (Int.add_zero _) ▸ (Int.add_lt_add_left hpos _)
-
-def do_simple_loop {α : Type} [SimpleLoopState α] (s : α) : α :=
-  if hlt : SimpleLoopState.cur s < SimpleLoopState.finish s then
-  do_simple_loop (SimpleLoopState.adv s hlt) else s
-termination_by
-  int32_toNat_for_term (SimpleLoopState.finish s) -
-  int32_toNat_for_term (SimpleLoopState.cur s)
-decreasing_by
-  exact simple_loop_term s hlt
-
--- Once the loop is complete, 'finish' ≤ 'cur'
-theorem simple_loop_index_ge {α : Type} [SimpleLoopState α] (s : α) :
-  SimpleLoopState.finish s ≤ SimpleLoopState.cur (do_simple_loop s) := by
-  unfold do_simple_loop
-  split_ifs with h
-  · convert simple_loop_index_ge (SimpleLoopState.adv s h) using 1
-    exact (SimpleLoopState.hfinish s h).symm
-  · apply Int32.le_iff_toInt_le.mpr (Int.le_of_not_gt _)
-    contrapose! h
-    exact Int32.lt_iff_toInt_lt.mpr h
-termination_by
-  int32_toNat_for_term (SimpleLoopState.finish s) -
-  int32_toNat_for_term (SimpleLoopState.cur s)
-decreasing_by
-  exact simple_loop_term s h
-
--- Prove that a property is true for the result of the loop
--- given that it is invariant across the loop and true of the
--- initial state.
-theorem simple_loop_prop_const {α : Type} [SimpleLoopState α] (s : α)
-  (prop : α → Prop) (base : prop s)
-  (step : ∀ t hlt, prop t → prop (SimpleLoopState.adv t hlt)) :
-  prop (do_simple_loop s) := by
-  unfold do_simple_loop
-  split_ifs with h
-  · exact simple_loop_prop_const _ prop (step s h base) step
-  · exact base
-termination_by
-  int32_toNat_for_term (SimpleLoopState.finish s) -
-  int32_toNat_for_term (SimpleLoopState.cur s)
-decreasing_by
-  exact simple_loop_term s h
-
--- Elements which are unmodified by advancing the loop
--- are unmodifed by the full execution of the loop
--- This is a special case of 'prop_const' (above)
-theorem simple_loop_val_const {α β : Type} [SimpleLoopState α] (s : α)
-  (f : α → β) (hconst : ∀ t hlt, f (SimpleLoopState.adv t hlt) = f t) :
-  f (do_simple_loop s) = f s := by
-  let prop (t : α) : Prop := f t = f s
-  have base : f s = f s := rfl
-  apply simple_loop_prop_const s prop base
-  unfold prop
-  exact fun t hlt ht ↦ Eq.trans (hconst t hlt) ht
-
--- Specifically, 'finish' is unmodified by the loop's execution
-@[simp] theorem simple_loop_finish_const {α : Type} [SimpleLoopState α] (s : α) :
-  SimpleLoopState.finish (do_simple_loop s) = SimpleLoopState.finish s :=
-  simple_loop_val_const s SimpleLoopState.finish SimpleLoopState.hfinish
-
--- Specifically, 'inc' is unmodified by the loop's execution
-@[simp] theorem simple_loop_inc_const {α : Type} [SimpleLoopState α] (s : α) :
-  SimpleLoopState.inc (do_simple_loop s) = SimpleLoopState.inc s :=
-  simple_loop_val_const s SimpleLoopState.inc SimpleLoopState.hinc
-
--- If the initial value of 'cur' is less than 'finish', the final
--- value will be less than 'finish' + 'inc'
-theorem simple_loop_index_lt_of_lt {α : Type} [SimpleLoopState α] (s : α)
-  (curlt : SimpleLoopState.cur s < SimpleLoopState.finish s) :
-  (fun t ↦ SimpleLoopState.cur t < SimpleLoopState.finish t + SimpleLoopState.inc t)
-    (do_simple_loop s) := by
-  let prop : α → Prop :=
-    fun t ↦ SimpleLoopState.cur t < SimpleLoopState.finish t + SimpleLoopState.inc t
-  have base : prop s := by
-    unfold prop
-    apply Int32.lt_trans curlt
-    apply Int32.lt_iff_toInt_lt.mpr
-    rw [simple_loop_state_toInt_finish_add_inc]
-    have hpos : (0 : ℤ) < _ := Int32.lt_iff_toInt_lt.mp (SimpleLoopState.hpos s)
-    convert (Int.add_zero _) ▸ (Int.add_lt_add_left hpos _)
-  have step : ∀ t hlt, prop t → prop (SimpleLoopState.adv t hlt) := by
-    unfold prop
-    intro t hlt h
-    rw [SimpleLoopState.hadv, SimpleLoopState.hfinish, SimpleLoopState.hinc]
-    apply Int32.lt_iff_toInt_lt.mpr
-    rw [simple_loop_state_toInt_finish_add_inc]
-    rw [simple_loop_state_toInt_cur_add_inc _ hlt]
-    exact Int.add_lt_add_right (Int32.lt_iff_toInt_lt.mp hlt) _
-  exact simple_loop_prop_const _ prop base step-/
+  exact loop_prop_const _ prop base step
